changed IsSet to Unique to maintain parity with ocaml-batteries, which F* draws from.

src/Flutterbye.Schedule.Core.fsi
@@ -1,6 +1,6 @@
 (*--build-config
-   options:--admit_fsi FStar.Seq --admit_fsi Flutterbye.Seq.IsSet;
-   other-files:seq.fsi Flutterbye.Seq.IsSet.fsi
+   options:--admit_fsi FStar.Seq --admit_fsi Flutterbye.Seq.Unique;
+   other-files:seq.fsi Flutterbye.Seq.Unique.fsi
 --*)
 
 // $legal:614:
@@ -26,7 +26,7 @@ module Flutterbye.Schedule.Core
    open Flutterbye
 
    type seq = FStar.Seq.seq
-   type SeqIsSet = Flutterbye.Seq.IsSet.IsSet
+   type Unique = Flutterbye.Seq.Unique.Unique
 
    type Name: Type
    type Effect: Type
@@ -35,6 +35,6 @@ module Flutterbye.Schedule.Core
    val empty: Schedule
    val length: s:Schedule -> Tot nat
    //val to_seq: s:Schedule -> Tot (seq (Effect * State))
-   //val ls: s:Schedule -> Tot (s:(seq Name){SeqIsSet s})
+   //val ls: s:Schedule -> Tot (s:(seq Name){Unique s})
 
 // $vim-fst:32: vim:set sts=3 sw=3 et ft=fstar:,$
